---
layout: single
title:  "확률론 기초 - 3강"
categories: boostcamp-math
sidebar:
  nav: "docs"
---

# 23/11/09 학습 내용

<h2>학습목표</h2>

확률의 non-naïve한 정의의 공리를 이용하여 확률의 특성을 증명할 수 있으며, 포함배제의 원리를 이해한다.

<h2>핵심 키워드</h2>

- Birthday problem
- 확률의 non-naïve한 정의의 공리
- 확률의 특성
- 포함배제의 원리

<h2>Lecture 3: Birthday Problem, Properties of Probability</h2>
3강- Birthday Problem과 확률의 특성

- Intro<br><br>
: : One of the most famous problems in statistics - Birthday Problem
: : K people, find the probability that 2 have the same birthday (not a specific day)<br><br>
: \<Assumptions>
: : Exclude February 29th (Exclude the leap year), 
: : assume other 365 days are equally likely, 
: : assume independence of births<br><br>
: : if <i>k > 365</i>, P is 1 (pigeonhole principle)
: : \[&emsp;o&emsp;](Jan 1), \[&emsp;o&emsp;](Jan 2), ... , \[&emsp;oo&emsp;](Dec 31)
: : if <i>k ≤ 365</i>
: (The answer is **23** people (Counter-intuitively small answer))
: : P(no match) = 365 · 364 · 363 ·  ... · (365 - k + 1) / 365<sup>k</sup>
: : If we compute the above formula, 
: : P(match) ≈ {50.7%, if k = 23}, {97%, if k = 50}, {99.999%, if k = 100}
: : It's not that intuitive
: : <sub>k</sub>C<sub>2</sub> = k·(k-1) / 2
: : <sub>23</sub>C<sub>2</sub> = 253 (253 pairs of people out of 23 people -> It seems more plausible)
: : If the birthday is same or off by one day, **k = 14**
: : <span style="color:red">(궁금증) 23명이 있으면 생일 같은 사람 둘이 있을 확률이 50.7%라고 하는데, 그게 내 생일일 확률은 얼마나 될까? 50 / 23 %?(경험적으로 잘 겪어보지 못한 것 같음. 그래서 이게 더 직관적이지 않게 느껴지는 건 아닐까?)</span>
: <span style="color:red">=> 이건 오히려 여집합의 문제로 접근해야 한다. 나머지 사람들에 대해 나와 생일이 한 명도 겹치지 않을 확률을 계산해야 하고, 사람 수 n이라 할 때 1 - (364 / 365)<sup>n</sup> 이 되는 것이다!</span>

- Non-naive definition of Probability <br><br>
: : <u>2 Axioms</u>
: - (1) P(∅) = 0, P(S) = 1 <span style="color:lightgray">(S = Sample space (all possible outcomes))</span>
: - (2) P(<sub>n=1</sub>⋃<sub>∞</sub>A<sub>n</sub>) = <sub>n=1</sub>∑<sub>∞</sub>P(A<sub>n</sub>)<br>
(True if A<sub>1</sub>, A<sub>2</sub>, ... , A<sub>n</sub> are disjoint events = non-overlapping)
: : <u>Properties</u>
: - (1) P(A<sup>C</sup>) = 1 - P(A)<br>
<span style="color:gray">(Proof) 1 = P(S) = P(A ⋃ A<sup>C</sup>) = P(A) + P(A<sup>C</sup>) since A ⋂ A<sup>C</sup> = ∅</span>
: - (2) If A ⊆ B, then P(A) ≤ P(B)<br>
<span style="color:gray">(Proof) B = A ⋃ (B ⋂ A<sup>C</sup>), disjoint<br>
&emsp;&emsp;&emsp;P(B) = P(A) + P(B ⋂ A<sup>C</sup>) ≥ P(A)</span>
: - (3) P(A ⋃ B) = P(A) + P(B) - P(A ⋂ B)<br>
<span style="color:gray">(Proof) "disjointification"<br>
&emsp;&emsp;&emsp;P(A ⋃ (B ⋂ A<sup>C</sup>)) = P(A) + P(B ⋂ A<sup>C</sup>)<br>
&emsp;&emsp;&emsp;=(?) P(A) + P(B) - P(A ⋂ B), equivalent to P(A ⋂ B) + P(B ⋂ A<sup>C</sup>) = P(B) (<i>P(A) 지워지고 - P(A ⋂ B)이항한 것</i>)<br>
&emsp;&emsp;&emsp;Above is immediate by axiom two since (A ⋂ B), (A<sup>C</sup> ⋂ B) are disjoint and their union is B (Because we split B into two parts)</span>
: - P(A ⋃ B ⋃ C) = P(A) + P(B) + P(C) - P(A ⋂ B) - P(A ⋂ C) - P(B ⋂ C) + P(A ⋂ B ⋂ C)
: - P (A<sub>1</sub> ⋃ A<sub>2</sub> ⋃, ... ,A<sub>n</sub>) = <sub>j=1</sub>Σ<sub>n</sub>P(A<sub>j</sub>) - <sub>i<j</sub>Σ P(A<sub>i</sub> ⋂ A<sub>j</sub>) + <sub>i<j<k</sub>Σ P(A<sub>i</sub> ⋂ A<sub>j</sub> ⋃ A<sub>k</sub>) - ... + (-1)<sup>n+1</sup> · P(A<sub>1</sub> ⋂ A<sub>2</sub>, ... ,A<sub>n</sub>)
: <br><b>- DeMontmort's Problem (1713) (matching problem)</b>
: <span style="color:red;font-size:8pt"><i>(아직 잘 이해가 안 돼서, 한 번 더 봐야겠다)</i></span><br><br>
: : We have a deck of cards, having number from 1 to n
: : n cards, labeled 1, 2, ... , n
: : If one of the cards' number matches its position in the deck, the player wins.
: : Let A<sub>j</sub> be the event, "j<sub>th</sub> card matches"
: : P(A<sub>1</sub> ⋃ A<sub>2</sub> ⋃, ... ,⋃ A<sub>n</sub>)
: : Let's take advantage of symmetry.<br><br>
: : P(A<sub>j</sub>) = 1 / n, since all positions are equally likely for the card labeled j.
: : P(A<sub>1</sub> ⋂ A<sub>2</sub>) = (n - 2)! / n! = 1 / n · (n - 1)
: : P(A<sub>1</sub> ⋂, ... ,⋂ A<sub>k</sub>) = (n-k)! / n!
: : P(A<sub>1</sub> ⋃ A<sub>2</sub> ⋃, ... ,⋃ A<sub>n</sub>) = n · 1 / n - n · (n - 1) / 2! · 1 / n · (n - 1) + n · (n - 1) · (n - 2) / 3! · 1 / n · (n - 1) · (n - 2) - ...
: = 1 - 1 / 2! + 1 / 3! - 1 / 4! + ... + (-1)<sup>n+1</sup> · 1 / n!<br>
: : <span style="color:red">이 사이 과정이 어떻게 되는 거? (Taylor series for e to the x?)</span><br>
: : <span style="color:red">(강의 설명) "That's exactly the Taylor series for e to the x evaluated at x equals minus 1"</span><br>
<b>≈ 1 - 1 / e</b>
: : <span style="color:gray">this is the answer!</span>
